rocq-skylabs-brick/tests/cpp_prog.v
@@ -2,7 +2,6 @@ Require Import skylabs.lang.cpp.parser.
 Require Import skylabs.lang.cpp.parser.plugin.cpp2v.
 
 cpp.prog module
-  abi Little
   defns (parser.Dtype "align_val_t") (parser.Dtypedef "xx" (Tnamed "align_val_t")).
 
 Print module.
