rocq-skylabs-brick/theories/lang/cpp/syntax/abi.v
@@ -1,0 +1,49 @@
+(*
+ * Copyright (c) 2020-2026 BlueRock Security, Inc.
+ * This software is distributed under the terms of the BedRock Open-Source License.
+ * See the LICENSE-BedRock file in the repository root for details.
+ *)
+
+Require Export elpi.apps.NES.NES.
+Require Import stdpp.fin_maps.
+Require Import skylabs.prelude.base.
+Require Import skylabs.prelude.avl.
+Require Import skylabs.prelude.lens.
+Require Import skylabs.prelude.elpi.derive.
+Require Import skylabs.prelude.elpi.derive.lens.
+Require Import skylabs.prelude.pstring.
+Require Import skylabs.lang.cpp.syntax.core.
+Require Import skylabs.lang.cpp.syntax.types.
+Require Import skylabs.lang.cpp.syntax.decl.
+Require Import skylabs.lang.cpp.syntax.namemap.
+
+(** This record contains implementation-defined information about a translation unit that is chosen by our clang.
+https://eel.is/c++draft/defns.impl.defined#def:behavior,implementation-defined
+
+TODO: maybe just ABI because we're in the context of C++.
+*)
+NES.Begin abi.
+  Record t : Set := mkT
+  { uintptr_t_rank : int_rank.t
+    (* ^ the size of a pointer *)
+  ; char_signed : signed
+    (* ^ whether or not `char` is signed or unsigned *)
+  ; wchar_signed : signed
+  ; byte_order : endian
+  }.
+  #[only(lens,eq_dec)] derive t.
+
+  Definition uintptr_t_type (info : t) : type :=
+    Tnum info.(uintptr_t_rank) Unsigned.
+  Definition pointer_size_bitsize (info : t) : bitsize :=
+    int_rank.bitsize info.(uintptr_t_rank).
+
+  (** Common Linux ABIs. Just for testing. *)
+
+  Definition x64_linux : t :=
+    mkT int_rank.Ilong Signed Signed Little.
+  Definition armle64_linux : t :=
+    mkT int_rank.Ilong Unsigned Unsigned Little.
+
+  Definition abi_default : t := x64_linux.
+NES.End abi.
